src/ndep/SymEvalTests.v
@@ -1,0 +1,156 @@
+Require Import List DepList.
+Require Import Heaps.
+Require Import Bedrock.ndep.Expr Bedrock.ndep.SepExpr Bedrock.ndep.SymEval.
+
+Module EvaluatorTests (B : Heap) (ST : SepTheoryX.SepTheoryXType B).
+  Module Import SE := Evaluator B ST.
+
+  Section Tests.
+    Variable a b : Type.
+
+    Variable ptsto32 : B.addr -> W -> ST.hprop a b nil.
+
+    Ltac isConst e :=
+      match e with
+        | true => true
+        | false => true
+        | O => true
+        | S ?e => isConst e
+        | _ => false
+      end.
+
+    Definition addr_type : Expr.type :=
+      {| Expr.Impl := B.addr 
+       ; Expr.Eq := fun x y => match B.addr_dec x y with
+                                 | left pf => Some pf
+                                 | right _ => None
+                               end
+       |} .
+
+    Definition W_type : Expr.type :=
+      {| Expr.Impl := W
+       ; Expr.Eq := fun x y => match equiv_dec x y with
+                                 | left pf => Some pf
+                                 | right _ => None
+                               end
+       |}.
+
+    Definition a_type : Expr.type :=
+      {| Expr.Impl := a 
+       ; Eq := fun _ _ => None
+       |}.   
+    Definition b_type : Expr.type :=
+      {| Expr.Impl := b
+       ; Eq := fun _ _ => None
+       |}.   
+
+    Require Import Word.
+
+    Definition pre_types : list Expr.type := 
+      a_type :: b_type :: addr_type :: W_type :: nil.
+
+    Definition sfuncs : list (SEP.ssignature (wtypes pre_types 2 3) (tvType 0) (tvType 1)) :=
+      {| SDomain := tvType 2 :: tvType 3 :: nil
+       ; SDenotation := ptsto32 : functionTypeD
+         (map (tvarD (wtypes pre_types 2 3)) (tvType 2 :: tvType 3 :: nil))
+         (ST.hprop (tvarD (wtypes pre_types 2 3) (tvType 0))
+           (tvarD (wtypes pre_types 2 3) (tvType 1)) nil)
+       |} :: nil.
+    
+    Definition Satisfies cs stn (P : ST.hprop a b nil) m : Prop :=
+      exists sm, 
+          ST.satisfies cs P stn sm
+       /\ ST.HT.satisfies sm m.
+
+    Theorem addr_not_state : 3 <> 2.
+      clear; auto.
+    Qed.
+
+    Definition known : list nat := 0 :: nil.
+
+    Definition evaluators : DepList.hlist (fun n : nat => match nth_error sfuncs n with
+                                                            | None => Empty_set 
+                                                            | Some ss => 
+                                                              SymEval_word pre_types addr_not_state
+                                                                (pcIndex := 0) (stateIndex := 1) ss
+                                                          end) known.
+      refine (DepList.HCons _ DepList.HNil); simpl.
+      refine (
+        {| sym_read_word := fun _ args p => 
+           match args with
+             | p' :: v :: nil => 
+               if seq_dec p p' then Some v else None
+             | _ => None
+           end
+         ; sym_write_word := fun _ args p v =>
+           match args with
+             | p' :: v' :: nil => 
+               if seq_dec p p' then Some (p' :: v :: nil) else None
+             | _ => None
+           end
+         ; sym_read_word_correct := _
+         ; sym_write_word_correct := _
+         |}).
+      admit.
+      admit.
+    Defined.
+
+    Goal forall p1 p2 p3 v1 v2 v3 cs stn m,
+      Satisfies cs stn (ST.star (ptsto32 p1 v1) (ST.star (ptsto32 p2 v2) (ptsto32 p3 v3))) m
+      -> ST.HT.mem_get_word (IL.implode stn) p1 m = Some v1.
+    Proof.
+      intros.
+      match goal with
+        | [ H : Satisfies ?CS ?STN ?P ?M
+          |- context [ ST.HT.mem_get_word (IL.implode stn) ?PTR ?M ] ] =>
+        let Ts := constr:(@nil Type) in
+        let Ts := SEP.collectAllTypes_sexpr ltac:(isConst) Ts (P :: nil) in
+        let Ts := SEP.collectAllTypes_expr ltac:(isConst) Ts (PTR, tt) in
+        let types := eval unfold pre_types in pre_types in
+        let types := SEP.extend_all_types Ts types in
+        let sexprs := constr:(P :: nil) in
+        match SEP.reflect_sexprs a b ltac:(isConst) types tt tt sexprs with
+          | (?types, ?pcType, ?stateType, ?funcs, ?sfuncs, ?P :: nil) =>
+            match SEP.reflect_exprs ltac:(isConst) types funcs (PTR, tt) with
+              | (?types, ?funcs, ?PTR :: nil) => 
+                let hyps := constr:(@nil (expr pre_types)) in
+                let s := eval simpl in (SEP.hash P) in
+                generalize (@symeval_read_word_correct types 1 0 2 3 addr_not_state sfuncs known evaluators
+                  hyps PTR (snd s) _ (refl_equal _) CS STN funcs nil nil M I H)
+            end
+        end
+      end.
+      simpl. auto.
+    Qed.
+
+    Goal forall p1 p2 p3 v1 v2 v3 cs stn m,
+      Satisfies cs stn (ST.star (ptsto32 p1 v1) (ST.star (ptsto32 p2 v2) (ptsto32 p3 v3))) m
+      -> Satisfies cs stn (ST.star (ptsto32 p1 v1) (ST.star (ptsto32 p2 v3) (ptsto32 p3 v3))) 
+           (ST.HT.mem_set_word (IL.explode stn) p2 v3 m).
+    Proof.
+      intros.
+      match goal with
+        | [ H : Satisfies ?CS ?STN ?P ?M
+          |- context [ ST.HT.mem_set_word (IL.explode stn) ?PTR ?VAL ?M ] ] =>
+        let Ts := constr:(@nil Type) in
+        let Ts := SEP.collectAllTypes_sexpr ltac:(isConst) Ts (P :: nil) in
+        let Ts := SEP.collectAllTypes_expr ltac:(isConst) Ts (PTR, (VAL, tt)) in
+        let types := eval unfold pre_types in pre_types in
+        let types := SEP.extend_all_types Ts types in
+        let sexprs := constr:(P :: nil) in
+        match SEP.reflect_sexprs a b ltac:(isConst) types tt tt sexprs with
+          | (?types, ?pcType, ?stateType, ?funcs, ?sfuncs, ?P :: nil) =>
+             match SEP.reflect_exprs ltac:(isConst) types funcs (PTR, (VAL, tt)) with
+              | (?types, ?funcs, ?PTR :: ?VAL :: nil) => 
+                 let hyps := constr:(@nil (expr pre_types)) in
+                let s := eval simpl in (SEP.hash P) in
+                generalize (@symeval_write_word_correct types 1 0 2 3 addr_not_state sfuncs known evaluators 
+                  hyps PTR VAL (snd s) _ (refl_equal _) CS STN funcs nil nil M _ I (refl_equal _) H)
+            end
+        end
+      end.
+      simpl; auto.
+    Qed.
+
+  End Tests.
+End EvaluatorTests.
